projects/lib/gmp_proof_auto.v
@@ -243,3 +243,27 @@ Proof. Admitted.
 Lemma proof_of_mpz_realloc_partial_solve_wit_10 : mpz_realloc_partial_solve_wit_10.
 Proof. Admitted. 
 
+Lemma proof_of_mpz_sgn_safety_wit_1 : mpz_sgn_safety_wit_1.
+Proof. Admitted. 
+
+Lemma proof_of_mpz_sgn_safety_wit_2 : mpz_sgn_safety_wit_2.
+Proof. Admitted. 
+
+Lemma proof_of_mpz_sgn_safety_wit_3 : mpz_sgn_safety_wit_3.
+Proof. Admitted. 
+
+Lemma proof_of_mpz_sgn_safety_wit_4 : mpz_sgn_safety_wit_4.
+Proof. Admitted. 
+
+Lemma proof_of_mpz_sgn_safety_wit_5 : mpz_sgn_safety_wit_5.
+Proof. Admitted. 
+
+Lemma proof_of_mpz_sgn_partial_solve_wit_1 : mpz_sgn_partial_solve_wit_1.
+Proof. Admitted. 
+
+Lemma proof_of_mpz_sgn_partial_solve_wit_2 : mpz_sgn_partial_solve_wit_2.
+Proof. Admitted. 
+
+Lemma proof_of_mpz_sgn_partial_solve_wit_3 : mpz_sgn_partial_solve_wit_3.
+Proof. Admitted. 
+
